code/sha3/Hacl.Spec.SHA3.Vec.fst
@@ -16,40 +16,118 @@ open Spec.SHA3.Constants
 
 #reset-options "--z3rlimit 50 --max_fuel 0 --max_ifuel 0"
 
+val create5: #a:Type -> x0:a -> x1:a -> x2:a -> x3:a -> x4:a -> lseq a 5
+
+let create5 #a x0 x1 x2 x3 x4 =
+  let l = [x0; x1; x2; x3; x4] in
+  assert_norm (List.Tot.length l = 5);
+  createL l
+
+val create5_lemma: #a:Type -> x0:a -> x1:a -> x2:a -> x3:a -> x4:a ->
+  Lemma (let s = create5 x0 x1 x2 x3 x4 in
+    s.[0] == x0 /\ s.[1] == x1 /\ s.[2] == x2 /\ s.[3] == x3 /\ s.[4] == x4)
+  [SMTPat (create5 #a x0 x1 x2 x3 x4)]
+
+let create5_lemma #a x0 x1 x2 x3 x4 =
+  let l = [x0; x1; x2; x3; x4] in
+  assert_norm (List.Tot.length l = 5);
+  Seq.elim_of_list l
+
+val create25: #a:Type
+  -> x0:a -> x1:a -> x2:a -> x3:a -> x4:a -> x5:a -> x6:a -> x7:a
+  -> x8:a -> x9:a -> x10:a -> x11:a -> x12:a -> x13:a -> x14:a -> x15:a
+  -> x16:a -> x17:a -> x18:a -> x19:a -> x20:a -> x21:a -> x22:a -> x23:a
+  -> x24:a -> lseq a 25
+
+let create25 #a
+x0 x1 x2 x3 x4 x5 x6 x7 x8 x9 x10 x11 x12 x13 x14 x15
+x16 x17 x18 x19 x20 x21 x22 x23 x24 =
+  let l = [
+    x0; x1; x2; x3; x4; x5; x6; x7; x8; x9; x10; x11; x12; x13; x14; x15;
+    x16; x17; x18; x19; x20; x21; x22; x23; x24
+  ] in
+  assert_norm (List.Tot.length l = 25);
+  createL l
+
+val create25_lemma: #a:Type
+  -> x0:a -> x1:a -> x2:a -> x3:a -> x4:a -> x5:a -> x6:a -> x7:a
+  -> x8:a -> x9:a -> x10:a -> x11:a -> x12:a -> x13:a -> x14:a -> x15:a
+  -> x16:a -> x17:a -> x18:a -> x19:a -> x20:a -> x21:a -> x22:a -> x23:a
+  -> x24:a ->
+  Lemma (let s = create25 x0 x1 x2 x3 x4 x5 x6 x7 x8 x9 x10 x11 x12 x13 x14 x15 x16 x17 x18 x19 x20 x21 x22 x23 x24 in
+    s.[0] == x0 /\ s.[1] == x1 /\ s.[2] == x2 /\ s.[3] == x3 /\
+    s.[4] == x4 /\ s.[5] == x5 /\ s.[6] == x6 /\ s.[7] == x7 /\
+    s.[8] == x8 /\ s.[9] == x9 /\ s.[10] == x10 /\ s.[11] == x11 /\
+    s.[12] == x12 /\ s.[13] == x13 /\ s.[14] == x14 /\ s.[15] == x15 /\
+    s.[16] == x16 /\ s.[17] == x17 /\ s.[18] == x18 /\ s.[19] == x19 /\
+    s.[20] == x20 /\ s.[21] == x21 /\ s.[22] == x22 /\ s.[23] == x23 /\
+    s.[24] == x24)
+  [SMTPat (create25 #a x0 x1 x2 x3 x4 x5 x6 x7 x8 x9 x10 x11 x12 x13 x14 x15 x16 x17 x18 x19 x20 x21 x22 x23 x24)]
+
+let create25_lemma #a
+x0 x1 x2 x3 x4 x5 x6 x7 x8 x9 x10 x11 x12 x13 x14 x15
+x16 x17 x18 x19 x20 x21 x22 x23 x24 =
+  let l = [
+    x0; x1; x2; x3; x4; x5; x6; x7; x8; x9; x10; x11; x12; x13; x14; x15;
+    x16; x17; x18; x19; x20; x21; x22; x23; x24
+  ] in
+  assert_norm (List.Tot.length l = 25);
+  Seq.elim_of_list l;
+  of_list_index l 0
+
 unfold
-type state (m:m_spec) = lseq (element_t m) 25
+type state_spec (m:m_spec) = lseq (element_t m) 25
+
+noextract
+let state_spec_v (#m:m_spec) (s:state_spec m) : lseq (lseq uint64 25) (lanes m) =
+  createi #(lseq uint64 25) (lanes m) (fun i ->
+    create25 (vec_v s.[0]).[i] (vec_v s.[1]).[i] (vec_v s.[2]).[i]
+             (vec_v s.[3]).[i] (vec_v s.[4]).[i] (vec_v s.[5]).[i]
+             (vec_v s.[6]).[i] (vec_v s.[7]).[i] (vec_v s.[8]).[i]
+             (vec_v s.[9]).[i] (vec_v s.[10]).[i] (vec_v s.[11]).[i]
+             (vec_v s.[12]).[i] (vec_v s.[13]).[i] (vec_v s.[14]).[i]
+             (vec_v s.[15]).[i] (vec_v s.[16]).[i] (vec_v s.[17]).[i]
+             (vec_v s.[18]).[i] (vec_v s.[19]).[i] (vec_v s.[20]).[i]
+             (vec_v s.[21]).[i] (vec_v s.[22]).[i] (vec_v s.[23]).[i]
+             (vec_v s.[24]).[i])
+
+noextract
+let _C_v (#m:m_spec) (_C:lseq (element_t m) 5) : lseq (lseq uint64 5) (lanes m) =
+  createi #(lseq uint64 5) (lanes m) (fun i ->
+    create5 (vec_v _C.[0]).[i] (vec_v _C.[1]).[i] 
+            (vec_v _C.[2]).[i] (vec_v _C.[3]).[i] (vec_v _C.[4]).[i])
 
 unfold
 type index = n:size_nat{n < 5}
 
-let get (m:m_spec) (s:state m) (x:index) (y:index) : Tot (element_t m) =
+let get (m:m_spec) (s:state_spec m) (x:index) (y:index) : Tot (element_t m) =
   s.[x + 5 * y]
 
-let set (m:m_spec) (s:state m) (x:index) (y:index) (v:element_t m) : Tot (state m) =
+let set (m:m_spec) (s:state_spec m) (x:index) (y:index) (v:element_t m) : Tot (state_spec m) =
   s.[x + 5 * y] <- v
 
-let state_theta_inner_C (m:m_spec) (s:state m) (i:size_nat{i < 5}) (_C:lseq (element_t m) 5) : Tot (lseq (element_t m) 5) =
+let state_theta_inner_C (m:m_spec) (s:state_spec m) (i:size_nat{i < 5}) (_C:lseq (element_t m) 5) : Tot (lseq (element_t m) 5) =
   _C.[i] <- get m s i 0 ^| get m s i 1 ^| get m s i 2 ^| get m s i 3 ^| get m s i 4
 
-let state_theta0 (m:m_spec) (s:state m) (_C:lseq (element_t m) 5) =
+let state_theta0 (m:m_spec) (s:state_spec m) (_C:lseq (element_t m) 5) =
   repeati 5 (state_theta_inner_C m s) _C
 
-let state_theta_inner_s_inner (m:m_spec) (x:index) (_D:element_t m) (y:index) (s:state m) : Tot (state m) =
+let state_theta_inner_s_inner (m:m_spec) (x:index) (_D:element_t m) (y:index) (s:state_spec m) : Tot (state_spec m) =
   set m s x y (get m s x y ^| _D)
 
-let state_theta_inner_s (m:m_spec) (_C:lseq (element_t m) 5) (x:index) (s:state m) : Tot (state m) =
+let state_theta_inner_s (m:m_spec) (_C:lseq (element_t m) 5) (x:index) (s:state_spec m) : Tot (state_spec m) =
   let _D = _C.[(x + 4) % 5] ^| (_C.[(x + 1) % 5] <<<| (size 1)) in
   repeati 5 (state_theta_inner_s_inner m x _D) s
 
-let state_theta1 (m:m_spec) (s:state m) (_C:lseq (element_t m) 5) : Tot (state m) =
+let state_theta1 (m:m_spec) (_C:lseq (element_t m) 5) (s:state_spec m) : Tot (state_spec m) =
   repeati 5 (state_theta_inner_s m _C) s
 
-let state_theta (m:m_spec) (s:state m) : Tot (state m) =
+let state_theta (m:m_spec) (s:state_spec m) : Tot (state_spec m) =
   let _C = create 5 (zero_element m) in
   let _C = state_theta0 m s _C in
-  state_theta1 m s _C
+  state_theta1 m _C s
 
-let state_pi_rho_inner (m:m_spec) (i:size_nat{i < 24}) (current, s) : ((element_t m) & (state m)) =
+let state_pi_rho_inner (m:m_spec) (i:size_nat{i < 24}) (current, s) : ((element_t m) & (state_spec m)) =
   let r = keccak_rotc.[i] in
   let _Y = v keccak_piln.[i] in
   let temp = s.[_Y] in
@@ -58,32 +136,32 @@ let state_pi_rho_inner (m:m_spec) (i:size_nat{i < 24}) (current, s) : ((element_
   current, s
 
 val state_pi_rho_s: m:m_spec -> i:size_nat{i <= 24} -> Type0
-let state_pi_rho_s m i = (element_t m) & (state m)
+let state_pi_rho_s m i = (element_t m) & (state_spec m)
 
-let state_pi_rho (m:m_spec) (s_theta:state m) : Tot (state m) =
+let state_pi_rho (m:m_spec) (s_theta:state_spec m) : Tot (state_spec m) =
   let current = get m s_theta 1 0 in
   let _, s_pi_rho = repeat_gen 24 (state_pi_rho_s m)
     (state_pi_rho_inner m) (current, s_theta) in
   s_pi_rho
 
-let state_chi_inner0 (m:m_spec) (s_pi_rho:state m) (y:index) (x:index) (s:state m) : Tot (state m) =
+let state_chi_inner0 (m:m_spec) (s_pi_rho:state_spec m) (y:index) (x:index) (s:state_spec m) : Tot (state_spec m) =
   set m s x y
     (get m s_pi_rho x y ^|
      ((~| (get m s_pi_rho ((x + 1) % 5) y)) &|
       get m s_pi_rho ((x + 2) % 5) y))
 
-let state_chi_inner1 (m:m_spec) (s_pi_rho:state m) (y:index) (s:state m) : Tot (state m) =
+let state_chi_inner1 (m:m_spec) (s_pi_rho:state_spec m) (y:index) (s:state_spec m) : Tot (state_spec m) =
   repeati 5 (state_chi_inner0 m s_pi_rho y) s
 
-let state_chi (m:m_spec) (s_pi_rho:state m) : Tot (state m)  =
+let state_chi (m:m_spec) (s_pi_rho:state_spec m) : Tot (state_spec m)  =
   repeati 5 (state_chi_inner1 m s_pi_rho) s_pi_rho
 
-let state_iota (m:m_spec) (s:state m) (round:size_nat{round < 24}) : Tot (state m) =
+let state_iota (m:m_spec) (s:state_spec m) (round:size_nat{round < 24}) : Tot (state_spec m) =
   set m s 0 0 (get m s 0 0 ^| (load_element m (secret keccak_rndc.[round])))
 
 (* Equivalence *)
 
-let state_chi_inner (m:m_spec) (y:index) (s:state m) : Tot (state m) =
+let state_chi_inner (m:m_spec) (y:index) (s:state_spec m) : Tot (state_spec m) =
   let v0  = get m s 0 y ^| ((~| (get m s 1 y)) &| get m s 2 y) in
   let v1  = get m s 1 y ^| ((~| (get m s 2 y)) &| get m s 3 y) in
   let v2  = get m s 2 y ^| ((~| (get m s 3 y)) &| get m s 4 y) in
@@ -96,10 +174,10 @@ let state_chi_inner (m:m_spec) (y:index) (s:state m) : Tot (state m) =
   let s = set m s 4 y v4 in
   s
 
-let state_chi_equiv (m:m_spec) (s_pi_rho:state m) : Tot (state m)  =
+let state_chi_equiv (m:m_spec) (s_pi_rho:state_spec m) : Tot (state_spec m)  =
   repeati 5 (state_chi_inner m) s_pi_rho
 
-let state_chi_inner_equivalence0 (m:m_spec) (st_old:state m) (y:index) (st:state m) :
+let state_chi_inner_equivalence0 (m:m_spec) (st_old:state_spec m) (y:index) (st:state_spec m) :
   Lemma (requires (forall y'. (y' >= y /\ y' < 5) ==>
                    get m st_old 0 y' == get m st 0 y' /\
                    get m st_old 1 y' == get m st 1 y' /\
@@ -119,7 +197,7 @@ let state_chi_inner_equivalence0 (m:m_spec) (st_old:state m) (y:index) (st:state
          
          ()
 
-let state_chi_inner_equivalence1 (m:m_spec) (st_old:state m) (y:index) (st_new:state m) :
+let state_chi_inner_equivalence1 (m:m_spec) (st_old:state_spec m) (y:index) (st_new:state_spec m) :
   Lemma (requires (st_new == state_chi_inner m y st_old))
         (ensures (  (forall y'. (y' < 5 /\ y' > y) ==>
                     (get m st_new 0 y' == get m st_old 0 y' /\
@@ -129,7 +207,7 @@ let state_chi_inner_equivalence1 (m:m_spec) (st_old:state m) (y:index) (st_new:s
                      get m st_new 4 y' == get m st_old 4 y')))) = ()
 
 #push-options "--z3rlimit 50"
-let state_chi_equivalence (m:m_spec) (st_old:state m) :
+let state_chi_equivalence (m:m_spec) (st_old:state_spec m) :
   Lemma (state_chi_equiv m st_old == state_chi m st_old) =
          Lib.LoopCombinators.eq_repeati0 5 (state_chi_inner1 m st_old) st_old;
          Lib.LoopCombinators.unfold_repeati 5 (state_chi_inner1 m st_old) st_old 0;
@@ -173,27 +251,18 @@ let state_chi_equivalence (m:m_spec) (st_old:state m) :
 
 (* Equivalence *)
 
-let state_permute1 (m:m_spec) (round:size_nat{round < 24}) (s:state m) : Tot (state m) =
+let state_permute1 (m:m_spec) (round:size_nat{round < 24}) (s:state_spec m) : Tot (state_spec m) =
   let s_theta = state_theta m s in
   let s_pi_rho = state_pi_rho m s_theta in
   let s_chi = state_chi m s_pi_rho in
   let s_iota = state_iota m s_chi round in
   s_iota
 
-let state_permute (m:m_spec) (s:state m) : Tot (state m) =
+let state_permute (m:m_spec) (s:state_spec m) : Tot (state_spec m) =
   repeati 24 (state_permute1 m) s
 
 noextract
-let state_spec (m:m_spec) = lseq (element_t m) 25
-
-noextract
 let ws_spec (m:m_spec) = lseq (element_t m) 32
-
-noextract
-let state_spec_v (#a:keccak_alg) (#m:m_spec) (st:state_spec m) : lseq (words_state a) (lanes m) =
-  createi #(words_state a) (lanes m) (fun i ->
-    createi (state_word_length a) (fun j ->
-      (vec_v st.[j]).[i]))
 
 noextract
 let ws_spec_v (#a:keccak_alg) (#m:m_spec) (st:ws_spec m) : lseq (lseq (word a) 32) (lanes m) =
@@ -291,20 +360,20 @@ let load_ws (#a:keccak_alg) (#m:m_spec{is_supported m}) (b:multiblock_spec a m) 
   let ws = load_blocks #a #m b in
   transpose_ws #m ws
 
-let loadState_inner (m:m_spec) (ws:ws_spec m) (j:size_nat{j < 25}) (s:state m) : Tot (state m) =
+let loadState_inner (m:m_spec) (ws:ws_spec m) (j:size_nat{j < 25}) (s:state_spec m) : Tot (state_spec m) =
   s.[j] <- s.[j] ^| ws.[j]
 
 let loadState
   (#a:keccak_alg)
   (#m:m_spec{is_supported m})
   (b:multiblock_spec a m)
-  (s:state m) :
-  Tot (state m) =
+  (s:state_spec m) :
+  Tot (state_spec m) =
   let ws = load_ws b in
   repeati 25 (loadState_inner m ws) s
 
 noextract
-let storeState (#a:keccak_alg) (#m:m_spec{is_supported m}) (s:state m) :
+let storeState (#a:keccak_alg) (#m:m_spec{is_supported m}) (s:state_spec m) :
                 lseq uint8 (lanes m * 32 * word_length a) =
   let ws = create 32 (zero_element m) in
   let ws = update_sub ws 0 25 s in
@@ -351,7 +420,7 @@ let next_block (#m:m_spec{is_supported m})
 
 let absorb_next (#a:keccak_alg) (#m:m_spec{is_supported m})
                 (rateInBytes:size_nat{rateInBytes > 0 /\ rateInBytes <= 256})
-                (s:state m) : Tot (state m) =
+                (s:state_spec m) : Tot (state_spec m) =
   let nextBlock = next_block #m rateInBytes (next_block_seq_zero m) in
   let s = loadState #a #m nextBlock s in
   state_permute m s
@@ -401,8 +470,8 @@ val absorb_last:
   -> rateInBytes:size_nat{0 < rateInBytes /\ rateInBytes <= 256}
   -> rem:size_nat{rem < rateInBytes}
   -> input:multiseq (lanes m) 256
-  -> s:state m ->
-  Tot (state m)
+  -> s:state_spec m ->
+  Tot (state_spec m)
 
 let absorb_last #a #m delimitedSuffix rateInBytes rem input s =
   let lastBlock = load_last_block #m rem delimitedSuffix input in
@@ -417,8 +486,8 @@ let absorb_inner
   (#a:keccak_alg)
   (#m:m_spec{is_supported m})
   (b:multiblock_spec a m)
-  (s:state m) :
-  Tot (state m) =
+  (s:state_spec m) :
+  Tot (state_spec m) =
   let s = loadState b s in
   state_permute m s
 
@@ -456,8 +525,8 @@ let absorb_inner_block
   (inputByteLen:nat)
   (input:multiseq (lanes m) inputByteLen)
   (i:nat{i < inputByteLen / rateInBytes})
-  (s:state m) :
-  Tot (state m) =
+  (s:state_spec m) :
+  Tot (state_spec m) =
   let mb = get_multiblock_spec #m rateInBytes inputByteLen input i in
   absorb_inner #a #m mb s
 
@@ -467,8 +536,8 @@ let absorb_inner_nblocks
   (rateInBytes:size_nat{0 < rateInBytes /\ rateInBytes <= 256})
   (inputByteLen:nat)
   (input:multiseq (lanes m) inputByteLen)
-  (s:state m) :
-  Tot (state m) =
+  (s:state_spec m) :
+  Tot (state_spec m) =
   let blocks = inputByteLen / rateInBytes in
   let s = repeati blocks (absorb_inner_block #a #m rateInBytes inputByteLen input) s in
   s
@@ -476,44 +545,18 @@ let absorb_inner_nblocks
 let absorb
   (#a:keccak_alg)
   (#m:m_spec{is_supported m})
-  (s:state m)
+  (s:state_spec m)
   (rateInBytes:size_nat{0 < rateInBytes /\ rateInBytes <= 256})
   (inputByteLen:nat)
   (input:multiseq (lanes m) inputByteLen)
   (delimitedSuffix:byte_t) :
-  Tot (state m) =
+  Tot (state_spec m) =
 
   let s = absorb_inner_nblocks #a #m rateInBytes inputByteLen input s in
   let rem = inputByteLen % rateInBytes in
   let mb = get_multilast_spec #m rateInBytes inputByteLen input in
   let s = absorb_last #a #m delimitedSuffix rateInBytes rem mb s in
   s
-
-noextract
-let init_b1 (#m:m_spec{lanes m == 1})
-            (outputByteLen:size_nat) :
-            multiseq (lanes m) outputByteLen =
-  let l = create outputByteLen (u8 0) in
-  ntup1 l
-
-noextract
-let init_b4 (#m:m_spec{lanes m == 4})
-            (outputByteLen:size_nat) :
-            multiseq (lanes m) outputByteLen =
-  let l0 = create outputByteLen (u8 0) in
-  let l1 = create outputByteLen (u8 0) in
-  let l2 = create outputByteLen (u8 0) in
-  let l3 = create outputByteLen (u8 0) in
-  ntup4 (l0, (l1, (l2, l3)))
-
-(* Linked to impl but not used yet *)
-noextract
-let init_b (#m:m_spec{is_supported m})
-           (outputByteLen:size_nat) :
-           multiseq (lanes m) outputByteLen =
-  match lanes m with
-  | 1 -> init_b1 #m outputByteLen
-  | 4 -> init_b4 #m outputByteLen
 
 let store_block4
   (#m:m_spec{lanes m == 4})
@@ -583,6 +626,9 @@ let update_b4 (#m:m_spec{lanes m == 4})
               (i:size_nat{i < outputByteLen / rateInBytes})
               (b:multiseq (lanes m) outputByteLen):
               multiseq (lanes m) outputByteLen =
+  assert (i + 1 <= outputByteLen / rateInBytes);
+  assert ((i + 1) * rateInBytes <= outputByteLen);
+  assert (i * rateInBytes + rateInBytes <= outputByteLen);
   store_output4 #m outputByteLen (i * rateInBytes) rateInBytes block b
 
 noextract
@@ -640,7 +686,7 @@ let squeeze_inner
   (outputByteLen:size_nat)
   (i:size_nat{i < outputByteLen / rateInBytes})
   (s, b) :
-  ((state m) & (multiseq (lanes m) outputByteLen)) =
+  ((state_spec m) & (multiseq (lanes m) outputByteLen)) =
 
   let block = storeState #a #m s in
   let b = update_b #m block rateInBytes outputByteLen i b in
@@ -650,7 +696,7 @@ let squeeze_inner
 val squeeze_s: 
   m:m_spec -> rateInBytes:size_nat{0 < rateInBytes /\ rateInBytes <= 256} ->
   outputByteLen:size_nat -> i:size_nat{i <= outputByteLen / rateInBytes} -> Type0
-let squeeze_s m rateInBytes outputByteLen i = (state m) & (multiseq (lanes m) outputByteLen)
+let squeeze_s m rateInBytes outputByteLen i = (state_spec m) & (multiseq (lanes m) outputByteLen)
 
 let squeeze_nblocks
   (#a:keccak_alg)
@@ -658,7 +704,7 @@ let squeeze_nblocks
   (rateInBytes:size_nat{0 < rateInBytes /\ rateInBytes <= 256})
   (outputByteLen:size_nat)
   (s, b) :
-  ((state m) & (multiseq (lanes m) outputByteLen)) =
+  ((state_spec m) & (multiseq (lanes m) outputByteLen)) =
   let outBlocks = outputByteLen / rateInBytes in
   repeat_gen outBlocks (squeeze_s m rateInBytes outputByteLen)
     (squeeze_inner #a #m rateInBytes outputByteLen) (s, b)
@@ -666,7 +712,7 @@ let squeeze_nblocks
 let squeeze_last
   (#a:keccak_alg)
   (#m:m_spec{is_supported m})
-  (s:state m)
+  (s:state_spec m)
   (rateInBytes:size_nat{0 < rateInBytes /\ rateInBytes <= 256})
   (outputByteLen:size_nat)
   (b:multiseq (lanes m) outputByteLen) :
@@ -678,7 +724,7 @@ let squeeze_last
 let squeeze
   (#a:keccak_alg)
   (#m:m_spec{is_supported m})
-  (s:state m)
+  (s:state_spec m)
   (rateInBytes:size_nat{0 < rateInBytes /\ rateInBytes <= 256})
   (outputByteLen:size_nat)
   (b:multiseq (lanes m) outputByteLen) :
