code/sha3/Hacl.Spec.SHA3.Lemmas.fst
@@ -1,0 +1,35 @@
+module Hacl.Spec.SHA3.Lemmas
+
+open FStar.Mul
+open Lib.IntTypes
+open Lib.Sequence
+open Lib.IntVector
+open Lib.IntVector.Transpose
+
+open Spec.Hash.Definitions
+open Hacl.Spec.SHA3.Vec
+open Hacl.Spec.SHA3.Vec.Common
+
+#set-options "--z3rlimit 50 --fuel 0 --ifuel 1"
+
+val transpose_ws4_lemma_ij:
+  #m:m_spec{lanes m == 4} // lanes m * lanes m = 32
+  -> ws:ws_spec m
+  -> j:nat{j < lanes m}
+  -> i:nat{i < 32} ->
+  Lemma
+   (let l = lanes m in
+    (vec_v (transpose_ws4 ws).[i]).[j] == (vec_v ws.[i / l * l + j]).[i % l])
+
+let transpose_ws4_lemma_ij #m ws j i =
+  let l = lanes m in
+  let i_sub = i / l in
+  let j_sub = i % l in
+  assert (i_sub * l + j_sub == i);
+
+  let vs = sub ws (i_sub * l) l in
+  eq_intro (sub (transpose_ws4 ws) (i_sub * l) l) (transpose4x4_lseq vs);
+  assert ((vec_v (transpose_ws4 ws).[i]).[j] == (vec_v (transpose4x4_lseq vs).[j_sub]).[j]);
+  transpose4x4_lemma vs;
+  assert ((vec_v (transpose_ws4 ws).[i]).[j] == (vec_v vs.[j]).[j_sub]);
+  assert ((vec_v (transpose_ws4 ws).[i]).[j] == (vec_v ws.[i_sub * l + j]).[j_sub])
