lib/Lib.Buffer.fst
@@ -646,7 +646,7 @@ let create16 #w st v0 v1 v2 v3 v4 v5 v6 v7 v8 v9 v10 v11 v12 v13 v14 v15 =
   let h1 = ST.get () in
   assert (Seq.equal (as_seq h1 st) (Seq.create16 v0 v1 v2 v3 v4 v5 v6 v7 v8 v9 v10 v11 v12 v13 v14 v15))
 
-#set-options "--z3rlimit 50 --fuel 0 --ifuel 0"
+#set-options "--z3rlimit 300 --max_fuel 1"
 
 let create32 #w st v0 v1 v2 v3 v4 v5 v6 v7 v8 v9 v10 v11 v12 v13 v14 v15 v16 v17 v18 v19 v20 v21 v22 v23 v24 v25 v26 v27 v28 v29 v30 v31 =
   let h0 = ST.get () in
